%!TEX program = pdflatex
\documentclass{article}
\usepackage{amsmath}
\usepackage{bm}
\usepackage{array,tabularx} 
\usepackage{amssymb}
% \usepackage{txfonts}
\begin{document}

\begin{displaymath}
    \mathbf{Basic \quad Equation}
\end{displaymath}

\begin{displaymath}
    (a+b)^n = \sum_{k=0}^{n}\binom{n}{k}a^{n-k}b^{k} = \sum_{k=0}^n{C_{n}^{k}a^{n-k}b^k}
\end{displaymath}

\begin{displaymath}
    a^{n}-b^{n} = (a-b) \cdot \sum_{k=0}^{n-1}a^{n-1-k}b^{k}
\end{displaymath}

\begin{displaymath}
    \arcsin x + \arccos x = \arctan x + \mathrm{arccot}x = \frac{\pi}{2} 
\end{displaymath}

\begin{displaymath}
    f(x) = \int_{a}^{x}f'(t) \mathrm{d}t + f(a)
\end{displaymath}

\begin{displaymath}
    K = \frac{|y''x'-y'x''|}{(x'^{2}+y'^{2})^{\frac{3}{2}}}, \quad \rho = \frac{1}{K}
\end{displaymath}

\begin{displaymath}
    \int_{0}^{1} f(x) \mathrm{d}x = \sum_{i=1}^{n}\left(\frac{i+1}{n}-\frac{i}{n}\right)f\left(\frac{i}{n}\right) = \frac{1}{n}\sum_{i=1}^{n}f\left(\frac{2i+1}{2n}\right)
\end{displaymath} 

\begin{displaymath}
    \int_{t1}^{t2} f(x(t),y(t)) \mathrm{d}s = \int_{a}^{b} f(x,y(x)) \sqrt{x'^2+y'^2} \mathrm{d}x = \int_{\alpha}^{\beta} f(r,\theta)\sqrt{r^2 + r'^2} \mathrm{d}\theta
\end{displaymath}

\begin{displaymath}
    S = \int_{a}^{b}y(x)\mathrm{d}x = \int_{t1}^{t2}y(t)x'(t)\mathrm{d}t = \frac{1}{2}\int_{\alpha}^{\beta}{r^2(\theta)}\mathrm{d}\theta 
\end{displaymath}

\begin{displaymath}
    S_{side} = \int_{a}^{b}2 \pi y(x)\sqrt{x'^2(x)+y'^2(x)} \mathrm{d}x = \int_{\alpha}^{\beta}{2\pi r(\theta)\sin \theta \sqrt{r^2(\theta)+r'^2(\theta)}} \mathrm{d}\theta 
\end{displaymath}

\begin{displaymath} 
    V_{x} = \int_{a}^{b} \pi y^2(x)\mathrm{d}x \quad V_{y}= \int_{a}^{b}2\pi xy(x)\mathrm{d}x  
\end{displaymath}

\begin{align*} 
    \mathbf{1's \quad Taylor} \quad f(x) = \sum_{k=0}^{n}\frac{f^{(k)}(x)}{k!}x^{k} + R_{k+1}(\xi)
\end{align*}
\begin{align*} 
    \mathbf{2's \quad Taylor} \quad f(x,y) = f(x_{0},y_{0})+ f'_{x}(x_{0},y_{0})(x-x_{0}) + f'_{y}(x_{0},y_{0})(y-y_{0}) 
    \\ + \frac{1}{2}f''_{xy}(x_{0},y_{0})(x-x_{0})^2 + \frac{1}{2}f''_{yy}(x_{0},y_{0})(y-y_{0})^2 + \frac{1}{2}f''_{xy}(x_{0},y_{0})(x-x_{0})(y-y_{0}) + o(\rho) 
\end{align*}

\begin{displaymath} 
    \mathbf{important \quad integral \quad ABS }: \quad \int u \mathrm{d}u = \ln|u| + C 
\end{displaymath}

\begin{align*}
    \lim \mathbf{type} : \frac{0}{0} \quad \frac{\infty}{\infty} \quad 0 * \infty \quad \infty - \infty \quad \infty^{0} \quad 0^0 \quad 1^{\infty}
\end{align*}

\clearpage

\begin{align*}
    \mathbf{Multivariate \quad Integral} \\ 
    \iiint_{\Omega_{xyz}}f(x,y,z)\mathrm{d}x\mathrm{d}y\mathrm{d}z = \iiint_{\Omega_{uvw}}f(u,v,w)
        \begin{vmatrix}
            \frac{\partial x}{\partial u} & \frac{\partial x}{\partial v} & \frac{\partial x}{\partial w} \\
            \frac{\partial y}{\partial u} & \frac{\partial y}{\partial v} & \frac{\partial y}{\partial w} \\
            \frac{\partial z}{\partial u} & \frac{\partial z}{\partial v} & \frac{\partial z}{\partial w} \\
        \end{vmatrix}\mathrm{d}u\mathrm{d}v\mathrm{d}w\\ 
    \left.\frac{\partial f}{\partial l}\right|_{P_{0}=(x_{0},y_{0},z_{0})} = f_{x}(P_{0})\cos \alpha + f_{y}(P_{0})\cos \beta + f_{z}(P_{0})\cos \gamma\\
    \mathbf{\mathrm{grad}}f(x_{0},y_{0},z_{0}) = f_{x}(x_{0},y_{0},z_{0})\mathbf{\vec{i}} + f_{y}(x_{0},y_{0},z_{0})\mathbf{\vec{j}} + f_{z}(x_{0},y_{0},z_{0})\mathbf{\vec{k}} \\ 
    (\bar{x},\bar{y},\bar{z}) = \left(\frac{\iiint_{\Omega}x\rho \mathrm{d}v}{\iiint_{\Omega}\rho \mathrm{d}v},\frac{\iiint_{\Omega}y\rho \mathrm{d}v}{\iiint_{\Omega}\rho \mathrm{d}v},\frac{\iiint_{\Omega}z\rho \mathrm{d}v}{\iiint_{\Omega}\rho \mathrm{d}v}\right), \quad J_{k_{j}} = \iiint_{\Omega}((\sum_{i=1}^n{k_{i}^2})-k^2_{j})\rho\mathrm{d}v\\
    S = \iint_{\Sigma}\mathrm{d}S = \iint_{D_{xy}}\sqrt{1+\left(\frac{\partial z}{\partial x}\right)^2+\left(\frac{\partial z}{\partial y}\right)^2}\mathrm{d}x\mathrm{d}y \\ 
    S = \iint_{D_{zx}}\sqrt{1+\left(\frac{\partial y}{\partial z}\right)^2+\left(\frac{\partial y}{\partial x}\right)^2}\mathrm{d}z\mathrm{d}x = \iint_{D_{yz}}\sqrt{1+\left(\frac{\partial x}{\partial y}\right)^2+\left(\frac{\partial x}{\partial z}\right)^2}\mathrm{d}y\mathrm{d}z \\ 
    \iint_{-\Sigma}P\mathrm{d}y\mathrm{d}z+Q\mathrm{d}z\mathrm{d}x+R\mathrm{d}x\mathrm{d}y = -\iint_{\Sigma}P\mathrm{d}y\mathrm{d}z+Q\mathrm{d}z\mathrm{d}x+R\mathrm{d}x\mathrm{d}y \\  
    \oint_{\Sigma}P\mathrm{d}y\mathrm{d}z+Q\mathrm{d}z\mathrm{d}x+R\mathrm{d}x\mathrm{d}y = \iiint_{\Omega} \left(\frac{\partial P}{\partial x}+{\frac{\partial Q}{\partial y}}+{\frac{\partial R}{\partial z}}\right) \mathrm{d}v ,\quad \mathrm{div}\mathbf{\vec{A}} = \frac{\partial P}{\partial x}+{\frac{\partial Q}{\partial y}}+{\frac{\partial R}{\partial z}} \\
    \Sigma:F(x,y,z)=0 \quad \vec{n}=\left(\frac{F_{x}}{\sqrt{F_{x}^2+F_{y}^2+F_{z}^2}},\frac{F_{y}}{\sqrt{F_{x}^2+F_{y}^2+F_{z}^2}},\frac{F_{z}}{\sqrt{F_{x}^2+F_{y}^2+F_{z}^2}}\right) = (\cos \alpha,\cos \beta,\cos \gamma)\\
    \oint_{\Sigma}P\mathrm{d}y\mathrm{d}z+Q\mathrm{d}z\mathrm{d}x+R\mathrm{d}x\mathrm{d}y = \iint_{\Sigma}(P\cos \alpha+Q\cos \beta+R\cos \gamma )\mathrm{d}S\\  
    \oint_{\Gamma}P\mathrm{d}x+Q\mathrm{d}y +R\mathrm{d}z = \iint_{\Sigma}\left(\frac{\partial R}{\partial y}-\frac{\partial Q}{\partial z}\right)\mathrm{d}y\mathrm{d}z+\left(\frac{\partial P}{\partial z}-\frac{\partial R}{\partial x}\right)\mathrm{d}z\mathrm{d}x+\left(\frac{\partial Q}{\partial x}-\frac{\partial P}{\partial y}\right)\mathrm{d}x\mathrm{d}y \\
    \mathbf{\mathrm{rot}\vec{A}} = \left(\frac{\partial R}{\partial y}-\frac{\partial Q}{\partial z}\right)\mathbf{\vec{i}}+\left(\frac{\partial P}{\partial z}-\frac{\partial R}{\partial x}\right)\mathbf{\vec{j}}+\left(\frac{\partial Q}{\partial x}-\frac{\partial P}{\partial y}\right)\mathbf{\vec{k}}\\
    \iint_{\Sigma} f(x,y,z) \mathrm{d}z\mathrm{d}x = \iint_{\Sigma} -f(x,y,z) \mathrm{d}x\mathrm{d}z \quad \iint_{D}f(x,y)\mathrm{d}z\mathrm{d}x = \iint_{D}f(x,y)\mathrm{d}x\mathrm{d}z
\end{align*}

\clearpage 

\begin{align*}
    \mathbf{Gamma \quad Function \quad Integral} \\ 
    \left(-\frac{1}{2}\right)! = \sqrt{\pi} \\ 
    \left(\frac{2n+1}{2}\right)! = \left(\Pi_{i=n}^{0}{\frac{2i+1}{2}}\right)\sqrt{\pi} = \frac{2n+1}{2}\frac{2n-1}{2}\dots\frac{1}{2}\sqrt{\pi} \\ 
    \int_{0}^{\infty} x^{a}\mathrm{e}^{-x}\mathrm{d}x = a! \\
    \int_{0}^{\infty} x^{-\frac{1}{2}}\mathrm{e}^{-x}\mathrm{d}x = \sqrt{\pi}\\ 
    \int_{0}^{\infty} x^{3}\mathrm{e}^{-x}\mathrm{d}x = (3)! = 6 \\ 
    \int_{0}^{\infty} x^{\frac{5}{2}}\mathrm{e}^{-x}\mathrm{d}x = \frac{5}{2}\frac{3}{2}\frac{1}{2}\sqrt{\pi}\\  
    \int_{0}^{\infty} x^{a}\mathrm{e}^{-x^2}\mathrm{d}x = \frac{1}{2} \left(\frac{a-1}{2}\right)! \\ 
    \int_{0}^{\infty} x^{1}\mathrm{e}^{-x^2}\mathrm{d}x = \frac{1}{2} \left(\frac{1-1}{2}\right)! = \frac{1}{2} \\
    \int_{0}^{\infty} x^{4}\mathrm{e}^{-x^2}\mathrm{d}x = \frac{1}{2} \left(\frac{4-1}{2}\right)! = \frac{1}{2}\frac{3}{2}\frac{1}{2}\sqrt{\pi}\\ 
    \int_{0}^{\infty} x^{7}\mathrm{e}^{-x^2}\mathrm{d}x = \frac{1}{2} \left(\frac{7-1}{2}\right)! = \frac{1}{2}(3)! = 3\\
\end{align*}

\clearpage

\begin{align*}
    \mathbf{Infinite \quad Series} \\ 
    \lim_{n \to \infty} |\frac{a_{n+1}}{a_{n}}| = \rho \quad, R = \frac{1}{\rho} \\ 
    S(x) = \frac{a_{0}}{2} + \sum_{n=1}^{\infty}(a_{n}\cos{\frac{n\pi x}{l}} + b_{n}\sin{\frac{n\pi x}{l}}) \\ 
    a_{0} = \frac{1}{l}\int_{-l}^{l}f(x)\mathrm{d}x ,\quad a_{n} = \frac{1}{l}\int_{-l}^{l}f(x)\cos{\frac{n\pi x}{l}}\mathrm{d}x ,\quad b_{n} = \frac{1}{l}\int_{-l}^{l}f(x)\sin{\frac{n\pi x}{l}}\mathrm{d}x \\ 
    S(x) = \left\{ 
    \begin{array}{rl} 
        f(x),x \in consecutive \\ 
        \frac{f(x-0)+f(x+0)}{2},x \in discontinuity \\  
        \frac{f(l-0)+f(l+0)}{2},x = \{-l,l\} 
    \end{array} \right. \ \\ 
\end{align*}

\begin{align*}
    \mathbf{Constant \quad Series} \\  
    \sum_{k=1}^{\infty}{\frac{1}{k^2}} = \frac{\pi^2}{6} \quad \sum_{k=1}^{\infty}{\frac{1}{k^4}} = \frac{\pi^4}{90} \quad \sum_{k=1}^{\infty}{\frac{1}{k^6}} = \frac{\pi^6}{945} \\ 
    \sum_{i=0}^{n}{a_{i}} \cdot \sum_{j=0}^{n}{b_{j}} = \sum_{i=0}^{n}\sum_{j=0}^{n}{(a_{i} \cdot b_{j})} \quad \sum_{n=s}^{t}\ln{f(n)} = \ln{\prod_{n=s}^{t}}f(n) \\ 
    \sum_{i=0}^{n}{i} = \frac{n(n+1)}{2} \quad \sum_{i=1}^{n}i(i+1)(i+2)=\frac{n(n+1)(n+2)(n+3)}{4} \\ 
    \sum_{i=0}^{n}{i^2} = \frac{n(n+1)(2n+1)}{6} \quad \sum_{i=0}^{n}{i^3} = \left(\sum_{i=0}^{n}{i}\right)^2 = \frac{n^2(n+1)^2}{4} \\ 
    \sum_{i=1}^{\infty}{\frac{(-1)^{i+1}}{i}} = \sum_{i=0}^{\infty}{\frac{1}{(2i+1)(2i+2)}} = \sum_{i=1}^{\infty}{\frac{1}{2^i i}} = \sum_{i=1}^{\infty}({\frac{1}{3^i}+\frac{1}{4^i}})\frac{1}{i}= \ln2 \\ 
\end{align*}

\clearpage

\begin{align*}
    \mathbf{Power \quad Series} \\ 
    \sum_{n=0}^{\infty}{x^n} = \frac{1}{1-x} \\ 
    \sum_{n=0}^{\infty}{(-1)^nx^n} = \frac{1}{1+x} \\ 
    \sum_{n=1}^{\infty}{(-1)^{n-1}\frac{x^n}{n}} = \ln(1+x) \\ 
    \sum_{n=1}^{\infty}{\frac{x^n}{n}} = -\ln(1-x) \\ 
    \sum_{n=0}^{\infty}{(-1)^nx^{2n}} = \frac{1}{1+x^2} \\ 
    \sum_{n=0}^{\infty}{(-1)^{n}\frac{x^{2n+1}}{2n+1}} = \arctan x \\ 
    \sum_{n=0}^{\infty}{(n+1)x^n} = \frac{1}{(1-x)^2} \\ 
    \sum_{n=0}^{\infty}{(n+1)(n+2)x^n} = \frac{2}{(1-x)^3} \\
    \sum_{n=1}^{\infty}{\frac{x^{2n}}{n}} = -\ln(1-x^2) \\ 
    \sum_{n=0}^{\infty}{\frac{x^{2n+1}}{2n+1}} = \frac{1}{2}\ln(\frac{1+x}{1-x})\\  
    \sum_{n=0}^{\infty}{(-1)^{n} \frac{x^{2n+1}}{(2n+1)!}} = \sin x \\  
    \sum_{n=0}^{\infty}{(-1)^{n} \frac{x^{2n}}{(2n)!}} = \cos x \\  
    \sum_{n=0}^{\infty}{\frac{x^{n}}{n!}} =  \mathrm{e}^x \\ 
\end{align*}

\clearpage

\begin{align*}
    \mathbf{Basel \quad Problem} \\
    \sum_{n=1}^{\infty} \frac{1}{n^2} = \frac{\pi^2}{6} \\ 
    f(x) = x^2 \quad \underrightarrow{Fourier Expansion} \quad S(x) = \frac{a_{0}}{2}+\sum_{n=1}^{\infty}\left(a_{n}\cos nx+b_{n}\cos nx \right) \\
    a_{0} = \frac{2}{3}\pi^{2} \quad a_{n} = \frac{1}{\pi}\int_{-\pi}^{\pi} x^2 \cos nx \mathrm{d}x = (-1)^{n}\frac{4}{n^2}\\
    b_{n} = \frac{1}{\pi}\int_{-\pi}^{\pi} x^2 \sin nx \mathrm{d}x = 0 \\     
    S(x) = \frac{a_{0}}{2}+\sum_{n=1}^{\infty}a_{n}\cos nx= \frac{1}{3}\pi^{2} + \sum_{n=1}^{\infty}(-1)^{n}\frac{4}{n^2}\cos nx = \frac{1}{3}\pi^{2} + \sum_{n=1}^n\frac{4}{n^2} \\
    \exists x = 0, S(0) = \frac{1}{3}\pi^{2} + \sum_{n=1}^{\infty}(-1)^{n}\frac{4}{n^2} = f(0) = 0 \Longrightarrow \sum_{n=1}^{\infty}\frac{(-1)^{n-1}}{n^2} = \frac{\pi^{2}}{12}\\
    \exists x = \pi, S(\pi) = \frac{1}{3}\pi^{2} + \sum_{n=1}^{\infty}\frac{4}{n^2} = f(\pi) = \pi^2 \Longrightarrow \sum_{n=1}^{\infty}\frac{1}{n^2} = \frac{\pi^{2}}{6} \\ 
    \sum_{n=1}^{\infty}\frac{1}{(2n-1)^2} = \frac{\pi^{2}}{8} \quad \sum_{n=1}^{\infty}\frac{1}{(2n)^2} = \frac{\pi^{2}}{24} \\  
    \sum_{n=1}^{\infty}\left(\frac{1}{(2n-1)^2}+\frac{1}{(2n)^2}\right) = \sum_{n=1}^{\infty}{\frac{1}{n^2}} = \frac{\pi^{2}}{6}
\end{align*}

\begin{align*}
    \mathbf{Transcendental \quad Equation} \\ 
    \sum_{i=0}^{n}a_{i}x^i = 0 \Longrightarrow \prod_{i=0}^{n}(x-x_{i})=0 \\ 
    \prod_{i=0}^{n}x_{i} = (-1)^{n}\frac{a_{0}}{a_{n}},\quad \sum_{i=0}^{n}\frac{\prod_{i=0}^{n}x_{i}}{x_{i}} = (-1)^{n-1}\frac{a_{1}}{a_{n}} \\ 
    \sum_{i=0}^{n}\frac{1}{x_{i}} = -\frac{a_{1}}{a_{0}} \\ 
    \mathbf{eg.} \quad \tan x = x \Longrightarrow \sin{x} = \cos{x} \cdot x \\
    x - \frac{1}{6}x^3 + \frac{1}{120}x^5 +... = x \cdot (1-\frac{1}{2}x^2+\frac{1}{24}x^4+...) \\
    \frac{1}{3}x^3-\frac{1}{30}x^5+... = 0 \quad \underrightarrow{x \not= 0} \quad \frac{1}{3}x^2-\frac{1}{30}x^4+... = 0 \\
    \sum_{i=0}^{n}\frac{1}{t_{i}} = \frac{1}{10} \quad \underrightarrow{t = x^2} \quad \lim_{n \to \infty}\sum_{i=0}^{n}\frac{1}{x_{i}^2} = \frac{1}{10} 
\end{align*}

\clearpage

\end{document}