%!TEX program = pdflatex
\documentclass{article}
\usepackage{amsmath}
\usepackage{bm}
\usepackage{array,tabularx} 
\begin{document}
    
\begin{displaymath}
    \bm{Elementary \quad Function}
\end{displaymath}

\begin{displaymath}
    (a+b)^n = \sum_{k=0}^n{\bm{C_{n}^{k}}a^{n-k}b^k}
\end{displaymath}

\begin{displaymath}
    a^{n}-b^{n} = (a-b) \cdot \sum_{k=0}^{n-1}a^{n-1-k}b^{k}
\end{displaymath}

\begin{displaymath}
    \arcsin x + \arccos x = \arctan x + \mathrm{arccot}x = \frac{\pi}{2} 
\end{displaymath}

\begin{displaymath}
    f(x) = \int_{a}^{x}f'(t) \mathrm{d}t + f(a)
\end{displaymath}

\begin{displaymath}
    K = \frac{|y''x'-y'x''|}{(x'^{2}+y'^{2})^{\frac{3}{2}}}, \quad \rho = \frac{1}{K}
\end{displaymath}

\begin{displaymath}
    \int_{a}^{b} f(x) \mathrm{d}x = \lim_{\lambda \to 0} \sum_{i=1}^{n}f(\xi_{i})\Delta x_{i}
\end{displaymath} 

\begin{displaymath}
    \int_{t1}^{t2} f(x(t),y(t)) \mathrm{d}s = \int_{a}^{b} f(x,y(x)) \sqrt{x'^2+y'^2} \mathrm{d}x = \int_{\alpha}^{\beta} f(r,\theta)\sqrt{r^2 + r'^2} \mathrm{d}\theta ,\quad \theta = \alpha \to \beta
\end{displaymath}

\begin{displaymath}
    S = \int_{a}^{b}y(x)\mathrm{d}x = \int_{t1}^{t2}y(t)x'(t)\mathrm{d}t = \frac{1}{2}\int_{\alpha}^{\beta}{r^2(\theta)}\mathrm{d}\theta ,\quad \theta = \alpha \to \beta 
\end{displaymath}

\begin{displaymath}
    S_{side} = \int_{a}^{b}2 \pi y(x)\sqrt{x'^2(x)+y'^2(x)} \mathrm{d}x = \int_{\alpha}^{\beta}{2\pi r(\theta)\sin \theta \sqrt{r^2(\theta)+r'^2(\theta)}} \mathrm{d}\theta 
\end{displaymath}

\begin{displaymath}
    [\overrightarrow{abc}]= 
    \begin{vmatrix}
        a_{x} & a_{y} & a_{z} \\
        b_{x} & b_{y} & b_{z} \\
        c_{x} & c_{y} & c_{z} \\
    \end{vmatrix}
\end{displaymath}

\clearpage 

\begin{align*}
    \bm{Multivariate \quad Integral} \\ 
    \iiint_{\Omega_{xyz}}f(x,y,z)\mathrm{d}x\mathrm{d}y\mathrm{d}z = \iiint_{\Omega_{uvw}}f(u,v,w)
        \begin{vmatrix}
            \frac{\partial x}{\partial u} & \frac{\partial x}{\partial v} & \frac{\partial x}{\partial w} \\
            \frac{\partial y}{\partial u} & \frac{\partial y}{\partial v} & \frac{\partial y}{\partial w} \\
            \frac{\partial z}{\partial u} & \frac{\partial z}{\partial v} & \frac{\partial z}{\partial w} \\
        \end{vmatrix}\mathrm{d}u\mathrm{d}v\mathrm{d}w\\ 
    \left. \frac{\partial f}{\partial l}\right|_{P_{0}=(x_{0},y_{0},z_{0})} = f_{x}(P_{0})\cos \alpha + f_{y}(P_{0})\cos \beta + f_{z}(P_{0})\cos \gamma\\
    \bm{\mathrm{grad}}f(x_{0},y_{0},z_{0}) = f_{x}(x_{0},y_{0},z_{0})\bm{\vec{i}} + f_{y}(x_{0},y_{0},z_{0})\bm{\vec{j}} + f_{z}(x_{0},y_{0},z_{0})\bm{\vec{k}} \\ 
    (\bar{x},\bar{y},\bar{z}) = (\frac{\iiint_{\Omega}x\rho \mathrm{d}v}{\iiint_{\Omega}\rho \mathrm{d}v},\frac{\iiint_{\Omega}y\rho \mathrm{d}v}{\iiint_{\Omega}\rho \mathrm{d}v},\frac{\iiint_{\Omega}z\rho \mathrm{d}v}{\iiint_{\Omega}\rho \mathrm{d}v}), \quad J_{k_{j}} = \iiint_{\Omega}((\sum_{i=1}^n{k_{i}^2})-k^2_{j})\rho\mathrm{d}v\\
    S = \iint_{\Sigma}\mathrm{d}S = \iint_{D_{xy}}\sqrt{1+(\frac{\partial z}{\partial x})^2+(\frac{\partial z}{\partial y})^2}\mathrm{d}x\mathrm{d}y \\ 
    S = \iint_{D_{zx}}\sqrt{1+(\frac{\partial y}{\partial z})^2+(\frac{\partial y}{\partial x})^2}\mathrm{d}z\mathrm{d}x = \iint_{D_{yz}}\sqrt{1+(\frac{\partial x}{\partial y})^2+(\frac{\partial x}{\partial z})^2}\mathrm{d}y\mathrm{d}z \\ 
    \iint_{-\Sigma}P\mathrm{d}y\mathrm{d}z+Q\mathrm{d}z\mathrm{d}x+R\mathrm{d}x\mathrm{d}y = -\iint_{\Sigma}P\mathrm{d}y\mathrm{d}z+Q\mathrm{d}z\mathrm{d}x+R\mathrm{d}x\mathrm{d}y \\  
    \oint_{\Sigma}P\mathrm{d}y\mathrm{d}z+Q\mathrm{d}z\mathrm{d}x+R\mathrm{d}x\mathrm{d}y = \iiint_{\Omega} (\frac{\partial P}{\partial x}+{\frac{\partial Q}{\partial y}}+{\frac{\partial R}{\partial z}}) \mathrm{d}v ,\quad \mathrm{div}\bm{\vec{A}} = \frac{\partial P}{\partial x}+{\frac{\partial Q}{\partial y}}+{\frac{\partial R}{\partial z}} \\
    \Sigma:F(x,y,z)=0 \quad \vec{n}=(\frac{F_{x}}{\sqrt{F_{x}^2+F_{y}^2+F_{z}^2}},\frac{F_{y}}{\sqrt{F_{x}^2+F_{y}^2+F_{z}^2}},\frac{F_{z}}{\sqrt{F_{x}^2+F_{y}^2+F_{z}^2}}) = (\cos \alpha,\cos \beta,\cos \gamma)\\
    \oint_{\Sigma}P\mathrm{d}y\mathrm{d}z+Q\mathrm{d}z\mathrm{d}x+R\mathrm{d}x\mathrm{d}y = \iint_{\Sigma}(P\cos \alpha+Q\cos \beta+R\cos \gamma )\mathrm{d}S\\  
    \oint_{\Gamma}P\mathrm{d}x+Q\mathrm{d}y +R\mathrm{d}z = \iint_{\Sigma}(\frac{\partial R}{\partial y}-\frac{\partial Q}{\partial z})\mathrm{d}y\mathrm{d}z+(\frac{\partial P}{\partial z}-\frac{\partial R}{\partial x})\mathrm{d}z\mathrm{d}x+(\frac{\partial Q}{\partial x}-\frac{\partial P}{\partial y})\mathrm{d}x\mathrm{d}y \\
    \bm{\mathrm{rot}\vec{A}} = (\frac{\partial R}{\partial y}-\frac{\partial Q}{\partial z})\bm{\vec{i}}+(\frac{\partial P}{\partial z}-\frac{\partial R}{\partial x})\bm{\vec{j}}+(\frac{\partial Q}{\partial x}-\frac{\partial P}{\partial y})\bm{\vec{k}}\\
\end{align*}

\begin{align*}
    \bm{Infinite \quad Series} \\ 
    \lim_{n \to \infty} |\frac{a_{n+1}}{a_{n}}| = \rho \quad, R = \frac{1}{\rho} \\ 
    S(x) = \frac{a_{0}}{2} + \sum_{n=1}^{\infty}(a_{n}\cos{\frac{n\pi x}{l}} + b_{n}\sin{\frac{n\pi x}{l}}) \\ 
    a_{0} = \frac{1}{l}\int_{-l}^{l}f(x)\mathrm{d}x ,\quad a_{n} = \frac{1}{l}\int_{-l}^{l}f(x)\cos{\frac{n\pi x}{l}}\mathrm{d}x ,\quad b_{n} = \frac{1}{l}\int_{-l}^{l}f(x)\sin{\frac{n\pi x}{l}}\mathrm{d}x \\ 
    S(x) = \left\{ 
    \begin{array}{rl} 
        f(x),x \in consecutive \\ 
        \frac{f(x-0)+f(x+0)}{2},x \in discontinuity \\ 
        \frac{f(l-0)+f(l+0)}{2},x = \{-l,l\}
    \end{array} \right. \ \\ 
\end{align*}

\clearpage

\begin{align*}
    \bm{Traditional \quad Probability \quad Theory} \\ 
    A - B = A\bar{B} = A \cap \bar{B} \Rightarrow P(A-B) = P(A) - P(AB) \\ 
    f(x) = \frac{1}{\sqrt{2\pi}\sigma}\mathrm{e}^{-\frac{(x-\mu)^2}{2\sigma^2}} , x \in (-\infty,+\infty)  \\ 
    \Phi(x) = \int_{-\infty}^{x} f(t) \mathrm{d}t , X \sim N(0,1) ,\quad \Phi(a)+\Phi(-a) = 1, \quad F(x) = \Phi(\frac{x-\mu}{\sigma}) \\ 
    f_{X|Y}(x|y) = \frac{f(x,y)}{f_{Y}(y)}, f_{Y|X}(y|x) = \frac{f(x,y)}{f_{X}(x)}\\ 
    (X,Y) \sim U(D), 
    f(x,y) = \left\{ 
    \begin{array}{rl} 
        \frac{1}{S_{D}}, (x,y) \in D\\ 
        0, others
    \end{array} \right. \ \\ 
    (X,Y) \sim N(\mu_{1},\mu_{2};\sigma_{1},\sigma_{2},\rho),f(x,y) = \frac{1}{2\pi \sigma_{1} \sigma_{2} \sqrt{1-\rho^2}} \mathrm{e}^{-\frac{1}{2(1-\rho^2)}[(\frac{x-\mu_{1}}{\sigma_{1}})^2-\frac{2\rho (x-\mu_{1})(y-\mu_{2})}{\sigma_{1}\sigma_{2}}+(\frac{y-\mu_{2}}{\sigma_{2}})^2]} \\
\end{align*}

$\bm{Variable \quad Digital \quad Properties}$ \\ 
\begin{tabular}{|c|c|c|c|}%
    \hline 
    Distr & Mark & EX & DX \\ 
    \hline 
    Bin & B(n,p) & np & np(1-p) \\ 
    \hline 
    Poi & P($\lambda$) & $\lambda$ & $\lambda$ \\ 
    \hline 
    Geo & G(p) & $\frac{1}{p}$ & $\frac{1-p}{p^2}$ \\ 
    \hline 
    Hyp & H(n,M,N) & $\frac{nM}{N}$ & $\frac{nM}{N}(1-\frac{M}{N})(\frac{N-n}{N-1})$ \\ 
    \hline 
    Uni & U(a,b) & $\frac{a+b}{2}$ & $\frac{(b-a)^2}{12}$ \\ 
    \hline 
    Exp & $E(\lambda)$ & $\frac{1}{\lambda}$ & $\frac{1}{\lambda^2}$ \\ 
    \hline 
    Nor & $N(\mu,\sigma^2)$ & $\mu$ & $\sigma^2$ \\ 
    \hline 
\end{tabular}

\begin{align*}
    \bm{Large \quad Number \quad Law \quad Central \quad Limit \quad Theorem } \\ 
    P \{ {|X-E(X)|\ge \epsilon} \} \le \frac{D(X)}{\epsilon^{2}} \\
    \lim_{n \to \infty}P\{|\frac{X_{n}}{n}-p| < \epsilon\} = 1 \\
    \lim_{n \to \infty}P\{|\frac{1}{n}\sum_{k=1}^nx_{k}-\mu|<\epsilon\} = 1 \\
    \lim_{n \to \infty}P\{|\frac{1}{n}\sum_{k=1}^n X_{k} - \frac{1}{n}\sum_{k=1}^n E(X_{k})| < \epsilon\} = 1 \\ 
    \sum_{i=1}^{n}X_{i} \sim N(n\mu,n\sigma^2), \lim_{n \to \infty}P\{\frac{\sum_{i=1}^nX_{i}-n\mu}{\sqrt{n}\sigma} \le x\} = F_{n}(x) = \Phi(x) \\ 
    X \sim N(np,np(1-p)), \lim_{n \to \infty }P\{\frac{X_{n}-np}{\sqrt{np(1-p)}} \le x \} = \Phi(x) \\ 
\end{align*}

\clearpage
\begin{align*}
    \bm{Mathematical \quad Statistics} \\ 
    \bar{X} \sim N(\mu,\frac{\sigma^2}{n}), \frac{\bar{X}-u}{\sigma/\sqrt{n}} \sim N(0,1)\\ 
    S^2 = \frac{1}{n-1}\sum_{i=1}^n(X_{i}-\bar{X})^2 = \frac{1}{n-1}[\sum_{i=1}^nX_{i}^2 - n \bar{X}^2] \\ 
    E(S^2) = \sigma^2, D(S^2) = \frac{2\sigma^4}{n-1} \\ 
    \frac{\sum_{i=1}^n(X_{i}-\mu)^2}{\sigma^2} \sim \chi^2(n) \\ 
    \frac{\sum_{i=1}^n(X_{i}-\bar{X})^2}{\sigma^2} \sim \chi^2(n-1) \\ 
    \chi^2 \sim \chi^2(n), E(\chi^2(n)) = n, D(\chi^2(n)) = 2n \\ 
    T \sim t(n), T = \frac{X}{\sqrt{Y/n}} \frac{\sim}{\sim} \frac{N(0,1)}{\sqrt{\chi^2(n)/n}}\\
    F \sim F(n1,n2), F = \frac{X/n1}{Y/n2} \frac{\sim}{\sim} \frac{\chi^2(n1)/n1}{\chi^2(n2)/n2} \\ 
    (X,Y) \sim N(\mu_{1},\mu_{2};\sigma_{1}^2,\sigma_{2}^2,0) \\ 
    \frac{\frac{(n_{1}-1)S_{1}^2}{\sigma_{1}^2}/(n_{1}-1)}{\frac{(n_{2}-1)S_{2}^2}{\sigma_{2}^2}/(n_{2}-1)} \sim F(n_{1}-1,n_{2}-1) \\
    \frac{\frac{\sum_{i=1}^{n_{1}}(X_{i}-\mu_{1})^2}{\sigma_{1}^2}/n_{1}}{\frac{\sum_{i=1}^{n_{2}}(X_{i}-\mu_{2})^2}{\sigma_{2}^2}/n2} \sim F(n1,n2) \\  
    \frac{\bar{X}-\bar{Y}-(\mu_{1}-\mu_{2})}{\sqrt{\frac{\sigma_{1}^2}{n_{1}}+\frac{\sigma_{2}^2}{n2}}} \sim N(0,1) \\ 
    \exists \sigma_{1} = \sigma_{2}, \frac{\bar{X}-\bar{Y}-(\mu_{1}-\mu_{2})}{S_{\omega}\sqrt{\frac{1}{n_{1}}+\frac{1}{n_{2}}}} \sim t(n_{1}+n_{2}-2) \\ 
    S_{\omega} = \sqrt{\frac{(n_{1}-1)S_{1}^2+(n_{2}-1)S_{2}^2 }{n_{1}+n_{2}-2}}
\end{align*}

\clearpage

\begin{align*}
    \bm{Constant \quad Series} \\  
    \sum_{n=1}^{\infty}{\frac{(-1)^n}{2n-1}} = -\frac{\pi}{4} \\ 
    \sum_{k=1}^{\infty}{\frac{1}{k^2}} = \frac{\pi^2}{6} \quad \sum_{k=1}^{\infty}{\frac{1}{k^4}} = \frac{\pi^4}{90} \quad \sum_{k=1}^{\infty}{\frac{1}{k^6}} = \frac{\pi^6}{945} \\ 
    \sum_{i=0}^{n}{a_{i}} \cdot \sum_{j=0}^{n}{b_{j}} = \sum_{i=0}^{n}\sum_{j=0}^{n}{(a_{i} \cdot b_{j})} \quad \sum_{n=s}^{t}\ln{f(n)} = \ln{\prod_{n=s}^{t}}f(n) \\ 
    \sum_{i=0}^{n}{i} = \frac{n(n+1)}{2} \quad \sum_{i=0}^{n}{i^2} = \frac{n(n+1)(2n+1)}{6} \quad \sum_{i=0}^{n}{i^3} = (\sum_{i=0}^{n}{i})^2 = \frac{n^2(n+1)^2}{4} \\ 
    \sum_{i=1}^{\infty}{\frac{(-1)^{i+1}}{i}} = \sum_{i=0}^{\infty}{\frac{1}{(2i+1)(2i+2)}} = \sum_{i=1}^{\infty}{\frac{1}{2^i i}} = \sum_{n=1}^{\infty}({\frac{1}{3^i}+\frac{1}{4^i}})\frac{1}{i}= \ln2 \\ 
\end{align*}

\clearpage

\begin{align*}
    \bm{Power \quad Series} \\ 
    \sum_{n=0}^{\infty}{x^n} = \frac{1}{1-x} \\ 
    \sum_{n=0}^{\infty}{(-1)^nx^n} = \frac{1}{1+x} \\ 
    \sum_{n=1}^{\infty}{(-1)^{n-1}\frac{x^n}{n}} = \ln(1+x) \\ 
    \sum_{n=1}^{\infty}{\frac{x^n}{n}} = -\ln(1-x) \\ 
    \sum_{n=0}^{\infty}{(-1)^nx^{2n}} = \frac{1}{1+x^2} \\ 
    \sum_{n=0}^{\infty}{(-1)^{n}\frac{x^{2n+1}}{2n+1}} = \arctan x \\ 
    \sum_{n=0}^{\infty}{(n+1)x^n} = \frac{1}{(1-x)^2} \\ 
    \sum_{n=0}^{\infty}{(n+1)(n+2)x^n} = \frac{2}{(1-x)^3} \\
    \sum_{n=1}^{\infty}{\frac{x^{2n}}{n}} = -\ln(1-x^2) \\ 
    \sum_{n=0}^{\infty}{\frac{x^{2n+1}}{2n+1}} = \frac{1}{2}\ln(\frac{1+x}{1-x})\\  
    \sum_{n=0}^{\infty}{(-1)^{n} \frac{x^{2n+1}}{(2n+1)!}} = \sin x \\  
    \sum_{n=0}^{\infty}{(-1)^{n} \frac{x^{2n}}{(2n)!}} = \cos x \\  
    \sum_{n=0}^{\infty}{\frac{x^{n}}{n!}} =  \mathrm{e}^x \\ 
\end{align*}


\clearpage

\begin{align*}
    \bm{Transcendental \quad Equation} \\ 
    \sum_{i=0}^{n}a_{i}x^i = 0 \Longrightarrow \prod_{i=0}^{n}(x-x_{i})=0 \\ 
    \prod_{i=0}^{n}x_{i} = (-1)^{n}\frac{a_{0}}{a_{n}},\quad \sum_{i=0}^{n}\frac{\prod_{i=0}^{n}x_{i}}{x_{i}} = (-1)^{n-1}\frac{a_{1}}{a_{n}} \\ 
    \sum_{i=0}^{n}\frac{1}{x_{i}} = -\frac{a_{1}}{a_{0}} \\ 
    \bm{eg.} \quad \tan x = x \Longrightarrow \sin{x} = \cos{x} \cdot x \\
    x - \frac{1}{6}x^3 + \frac{1}{120}x^5 +... = x \cdot (1-\frac{1}{2}x^2+\frac{1}{24}x^4+...) \\
    \frac{1}{3}x^3-\frac{1}{30}x^5+... = 0 \quad \underrightarrow{x \not= 0} \quad \frac{1}{3}x^2-\frac{1}{30}x^4+... = 0 \\
    \sum_{i=0}^{n}\frac{1}{t_{i}} = \frac{1}{10} \quad \underrightarrow{t = x^2} \quad \lim_{n \to \infty}\sum_{i=0}^{n}\frac{1}{x_{i}^2} = \frac{1}{10} 
\end{align*}

\clearpage

\begin{align*}
    \bm{Beyond \quad Integral} \\
    \sum_{n=0}^\infty \frac{1}{(3n)!} \Longrightarrow S(x) = \sum_{n=0}^{\infty}{\frac{x^{3n}}{(3n)!}} ,S(1) = \frac{\mathrm{e}}{3}+\frac{2}{3}\cos\frac{\sqrt{3}}{2}\mathrm{e}^{-\frac{1}{2}}\\ 
    \iint_{D_{xy}}(\mathrm{e}^{x}\cos y)\mathrm{d}\sigma, D=\{(x,y)|x^2+y^2 \le 1\} \\ 
    \iint_{D_{xy}} (x+y)\mathrm{d}\sigma , D=\{(x,y)|y^2 \le x+2, x^2 \le y+2\} \\
    \bm{A_{0}} = \sum_{n=1}^\infty\frac{(-1)^{n-1}}{n}\sum_{m=0}^\infty\frac{1}{n2^m+1} \\
    \bm{A_{1}} = \int_{0}^{x^2} \pi(\sqrt[4]{1+t}-1)\sin t^4 \mathrm{d}x\\ 
    \bm{A_{2}} = \sum_{n=1}^\infty \frac{((n-1)!)^2(2t)^{2n}}{(2n)!} \\
    \bm{A_{3}} = \int_{0}^1\frac{(1-2x)\ln(1-x)}{x^2-x+1}\mathrm{d}x\\
    \bm{A_{4}} = x^2(x-\tan x)\ln(x^2+1)[(\frac{2\arctan \frac{y}{x}}{\pi})^y-1] \\ 
    \lim_{x \to 0^{+}} \lim_{y \to +\infty}\frac{\bm{A_{0}}\bm{A_{1}}}{\bm{A_{2}}\bm{A_{3}}\bm{A_{4}}} = \frac{27}{32}\\
\end{align*}

\begin{align*}
    \int\frac{\sec^3 x}{1-\tan^6 x}\mathrm{d}x \\
    \int\frac{1}{\csc x+\sec x+\tan x +\cot x}\mathrm{d}x \\ 
\end{align*}

\clearpage
\begin{displaymath}
    \lim_{N \to \infty}\sum_{n=1}^N\sum_{k=1}^n\frac{(-1)^{k-1}}{k}-\ln 2  = \ln 2-\frac{1}{2} \newline 
\end{displaymath}

\begin{displaymath}
    \lim_{n \to \infty}\sum_{i=1}^{n}\frac{1-\cos\frac{\pi}{\sqrt{n}}}{1+\cos\frac{i\pi}{\sqrt{2n}}}
\end{displaymath}
\begin{displaymath}
    \sum_{n=1 }^\infty\frac{(-1)^{[\sqrt{n}]}}{n}
\end{displaymath}

\begin{displaymath}
    t\frac{\mathrm{d}^3x}{\mathrm{d}t^3} + 3\frac{\mathrm{d}^2x}{\mathrm{d}t^2}-t\frac{\mathrm{d}x}{\mathrm{d}t}-x = 0
\end{displaymath}
\end{document}


    