%!TEX program = pdflatex
\documentclass{article}
\usepackage{amsmath}
\usepackage{bm}
\usepackage{array,tabularx} 
\usepackage{amssymb}
% \usepackage{txfonts}
\begin{document}

\begin{align*}
    \mathbf{Amazing \quad Integral \quad Sum \quad Limit} \\
    \lim_{n \to \infty}\sum_{k = 0}^{n}\sum_{i = 1}^{4}\frac{1}{(ik)!} \\
    \sum_{n=0}^{\infty} \frac{1}{n!}  \Longrightarrow S_{1}(x) = \sum_{n=0}^{\infty}\frac{x^n}{n!}, \quad S_{1}(1) = \mathrm{e}\\ 
    \sum_{n=0}^\infty \frac{1}{(2n)!} \Longrightarrow S_{2}(x) = \sum_{n=0}^{\infty}{\frac{x^{2n}}{(2n)!}}, \quad S_{2}(1) = \frac{\mathrm{e}^{-1}+\mathrm{e}}{2}\\\ 
    \sum_{n=0}^\infty \frac{1}{(3n)!} \Longrightarrow S_{3}(x) = \sum_{n=0}^{\infty}{\frac{x^{3n}}{(3n)!}} ,S_{3}(1) = \frac{\mathrm{e}}{3}+\frac{2}{3}\cos\left(\frac{\sqrt{3}}{2}\right)\mathrm{e}^{-\frac{1}{2}} \\ 
    \sum_{n=0}^{\infty} \frac{1}{(4n)!} \Longrightarrow S_{4}(x) = \sum_{n=0}^{\infty}{\frac{x^{4n}}{(4n)!}} ,S_{4}(1) = \frac{\mathrm{e}+\mathrm{e}^{-1}}{4}+\frac{\cos 1}{2} \\
    \lim_{n \to \infty}\sum_{k = 0}^{n}\sum_{i = 0}^{4}\frac{1}{(ik)!} = \frac{25}{12}\mathrm{e} + \frac{3}{4}\mathrm{e}^{-1}+\frac{2}{3}\cos\left(\frac{\sqrt{3}}{2}\right)\mathrm{e}^{-\frac{1}{2}} + \frac{\cos 1}{2}\\
    \iint_{D_{xy}} (x+y)\mathrm{d}\sigma , D=\{(x,y)|y^2 \le x+2, x^2 \le y+2\} \\
    \mathbf{A_{0}} = \sum_{n=1}^\infty\frac{(-1)^{n-1}}{n}\sum_{m=0}^\infty\frac{1}{n2^m+1} \\
    \mathbf{A_{1}} = \int_{0}^{x^2} \pi(\sqrt[4]{1+t}-1)\sin t^4 \mathrm{d}x\\ 
    \mathbf{A_{2}} = \sum_{n=1}^\infty \frac{((n-1)!)^2(2t)^{2n}}{(2n)!} \\
    \mathbf{A_{3}} = \int_{0}^1\frac{(1-2x)\ln(1-x)}{x^2-x+1}\mathrm{d}x\\
    \mathbf{A_{4}} = x^2(x-\tan x)\ln(x^2+1)[\left(\frac{2\arctan \frac{y}{x}}{\pi}\right)^y-1] \\ 
    \lim_{x \to 0^{+}} \lim_{y \to +\infty}\frac{\mathbf{A_{0}}\mathbf{A_{1}}}{\mathbf{A_{2}}\mathbf{A_{3}}\mathbf{A_{4}}} = \frac{27}{32}\\
\end{align*}

\begin{align*}
    \int\frac{\sec^3 x}{1-\tan^6 x}\mathrm{d}x \\
    \int\frac{1}{\csc x+\sec x+\tan x +\cot x}\mathrm{d}x \\ 
    \lim_{x \to 0 }\frac{-2\sin x+\arctan x-\frac{x^3 \cos x}{3}+\frac{\ln(\frac{1+x}{1-x})}{2}}{(\mathrm{e}^{x}-1)^2 \sum_{n=0}^{\infty}\left(1-\frac{1}{x^2}\right)^n D(\chi^2(x))} =  \frac{11}{40} 
\end{align*}

\begin{displaymath}
    \lim_{N \to \infty}\sum_{n=1}^N\sum_{k=1}^n\frac{(-1)^{k-1}}{k}-\ln 2  = \ln 2-\frac{1}{2} \newline 
\end{displaymath}

\begin{displaymath}
    \iint_{D}\mathrm{e}^{x}\cos y\mathrm{d}\sigma, D=\{(x,y)|x^2+y^2 \le 1\} \\  
\end{displaymath}

\begin{displaymath}
    \iint_{D}\mathrm{e}^{-y^{2}}\mathrm{d}x\mathrm{d}y,D = \{(x,y)|x < y < 1,0<x<1\}
\end{displaymath}
\begin{displaymath}
    \lim_{n \to \infty}\sum_{i=1}^{n}\frac{1-\cos\frac{\pi}{\sqrt{n}}}{1+\cos\frac{i\pi}{\sqrt{2n}}}
\end{displaymath}
\begin{displaymath}
    \sum_{n=1 }^\infty \frac{(-1)^{[\sqrt{n}]}}{n} \quad 
    \sum_{n=1}^{\infty} \frac{n!}{(2n+1)!!}\frac{1}{(n+1)} 
\end{displaymath}

\begin{displaymath}
    t\frac{\mathrm{d}^3x}{\mathrm{d}t^3} + 3\frac{\mathrm{d}^2x}{\mathrm{d}t^2}-t\frac{\mathrm{d}x}{\mathrm{d}t}-x = 0
\end{displaymath}

\begin{align*}
    X \sim F(x) \quad is \quad Consecutive \quad Variable : \int_{-\infty}^{+\infty}[F(x+a)-F(x)]\mathrm{d}x = a \\ 
\end{align*}

\begin{displaymath}
    \sum_{n=1}^{\infty} \frac{(-1)^n}{1+4n^2} = \frac{\pi}{2}\frac{1}{\mathrm{e}^{\frac{\pi}{2}}-\mathrm{e}^{-\frac{\pi}{2}}}-\frac{1}{2} \\ 
\end{displaymath}


\clearpage
\begin{align*}
    \mathbf{L} = \mathbf{L_{1}} + \mathbf{L_{2}} + \mathbf{L_{3}} + \mathbf{L_{4}} \\
    \mathbf{L_{1}} : x \in(0,1),y=0 \quad \mathbf{L_{2}} : y \in(0,1),x=1 \quad \mathbf{L_{3}} : x \in(1,0),y=1 \quad \mathbf{L_{4}} :  y \in(1,0),x = 0 \\
    I_{1} = \oint_{L}-xyf'_{x}(x,y)\mathrm{d}x + xyf_{y}'(x,y)\mathrm{d}y = \iint_{D}\left(\frac{\partial\left({xyf'_{y}(x,y)}\right) }{\partial x}-\frac{\partial\left(-{xyf'_{x}(x,y)}\right) }{\partial y}\right) \mathrm{d}x\mathrm{d}y \\ 
    = 2\iint_{D}xyf''_{xy}(x,y)\mathrm{d}x\mathrm{d}y+\iint_{D}\left(xf_{x}'(x,y)+yf_{y}'(x,y)\right)\mathrm{d}x\mathrm{d}y\\ 
    I_{1} = \oint_{L}-xyf'_{x}(x,y)\mathrm{d}x + xyf_{y}'(x,y)\mathrm{d}y = \int_{L_{1}}+\int_{L_{2}}+\int_{L_{3}}+\int_{L_{4}} \\
    = 0 + \int_{0}^{1}yf'_{y}(1,y)\mathrm{d}y+\int_{1}^{0}-xf'_{x}(x,1)\mathrm{d}x+0 \\ = \left. yf(1,y) \right|_{0}^{1}-\int_{0}^{1}f(1,y)\mathrm{d}y+\left. xf(x,1) \right|_{0}^{1}-\int_{0}^{1}f(x,1)\mathrm{d}x
    \\ = 0+0+0+0=0 \\
    I_{2} = \iint_{D}{xf'_{x}(x,y)+yf'_{y}(x,y)}\mathrm{d}x\mathrm{d}y=I_{3}-I_{4} \\  
    I_{3} = \oint_{L} -yf(x,y)\mathrm{d}x+xf(x,y)\mathrm{d}y = \iint_{D}\left(xf_{x}'(x,y)+yf_{y}'(x,y)\right)\mathrm{d}x\mathrm{d}y + 2\iint_{D}f(x,y)\mathrm{d}x\mathrm{d}y\\ 
    I_{3} = \oint_{L} -yf(x,y)\mathrm{d}x+xf(x,y)\mathrm{d}y = \int_{L_{1}}+\int_{L_{2}}+\int_{L_{3}}+\int_{L_{4}} \\
    = 0+\int_{0}^{1}f(1,y)\mathrm{d}y+\int_{1}^{0}-f(x,1)\mathrm{d}x+0 = 0+0+0+0=0 \\  
    I_{4} = 2\iint_{D}f(x,y)\mathrm{d}x\mathrm{d}y=2a\\
    I=\frac{1}{2}I_{1}-\frac{1}{2}I_{2} = \frac{1}{2}I_{1}-\frac{1}{2}(I_{3}-I_{4}) = 0-\frac{1}{2}(0-2a) = a \\   
\end{align*}


\clearpage
\begin{align*}
    \frac{1}{\log_{a}^3x}+\frac{1}{\log_{b}^3x}+\frac{1}{\log_{c}^3x} = \frac{3}{\log_{a}x\log_{b}x\log_{c}x}
    \\ (\log_{x}a)^3+(\log_{x}b)^3+(\log_{x}c)^3 = 3(\log_{x}a)(\log_{x}b)(\log_{x}c)
    \\ \aleph \quad \log_{x}a=m,\log_{x}b=n,\log_{x}c=p \rightarrow m^3+n^3+p^3 = 3mnp
    \\ \log_{a}x\log_{b}x\log_{c}x \neq 0 \longrightarrow mnp \neq 0
    % \\ (1). \exists p = 0 \rightarrow m^3+n^3=0 \rightarrow m = -n , p=0 \longrightarrow \log_{4}\left(\frac{a+b}{c}\right)=\frac{1}{2} 
    \\ \exists p \neq 0 \rightarrow (\frac{m}{p})^3+(\frac{n}{p})^3+1=3\frac{mn}{p^2}
    \\ \aleph \quad \frac{m}{p}=A,\frac{n}{p} =B \rightarrow A^3+B^3-3AB+1=0
    \\ \aleph \quad f(A,B) = A^3+B^3-3AB+1 = 0 
    \\ f_{A}'(A,B) = 3(A^2-B),f_{B}'{A,B}=3(B^2-A)
    \\ f_{AA}''(A,B)=6A,f_{BB}''(A,B)=6B,f_{AB}''(A,B)=-3
    \\ \exists f_{A}'(A,B)=f_{B}'(A,B) = 0 \longrightarrow A=B=1,f_{AA}''(A,B)f_{BB}''(1,1)>(f_{AB}''(1,1))^2
    \\ \exists only \quad A=B=1 \in \mathbf{R^2},f(A,B)=0 \longrightarrow f(A,B) = A^3+B^3-3AB+1 = 0 
    \\ so \quad \exists m = n = p = 1 \longrightarrow \log_{4}\left(\frac{a+b}{c}\right)=\frac{1}{2} 
\end{align*}

\clearpage


\begin{align*}
    X \sim N(0,1) \quad E(X^{2k}) = (2k-1)!! \quad E(X^{2k-1}) = 0 \\ 
    X \sim N(0,\sigma^2),Y \sim N(0,2\sigma^2) \\ 
    \frac{X}{\sigma} \sim N(0,1) \frac{Y}{\sqrt{2}\sigma} \sim N(0,1) \\ 
    \mathbf{My \quad Method} \\ 
    E(\left(\frac{X}{\sigma}\right)^4) = 3 , E(\left(\frac{X}{\sigma}\right)^2) = 1 \\ 
    E(\left(\frac{Y}{\sqrt{2}\sigma}\right)^4) = 3 , E(\left(\frac{Y}{\sqrt{2}\sigma}\right)^2) = 1 \\ 
    E(X^4) = 3\sigma^4 , E(X^2) = \sigma^2 , D(X^2) = 2\sigma^4 \\
    E(Y^4) = 12\sigma^4 , E(Y^2) = 2\sigma^2 , D(Y^2) = 8\sigma^4 \\
    D(\hat{\sigma}^2) = D(\frac{1}{2n}\sum_{i=1}^nX_{i}^2+\frac{1}{4n}\sum_{i=1}^nY_{i}^2) = \frac{1}{4n^2}\sum_{i=1}^{n}D(X_{i}^2)+\frac{1}{16n^2}\sum_{i=1}^{n}D(Y_{i}^2) = \frac{\sigma^4}{n}
    \\
    \mathbf{Answer Method}  \\ 
    (\frac{X}{\sigma})^2 \sim \chi^2{(1)} , (\frac{Y}{\sqrt{2}\sigma})^2 \sim \chi^2{(1)}\\  
    D(X^2) = 2\sigma^4  , D(Y^2) = 8\sigma^4 \\ 
    D(\hat{\sigma}^2) = D(\frac{1}{2n}\sum_{i=1}^nX_{i}^2+\frac{1}{4n}\sum_{i=1}^nY_{i}^2) = \frac{1}{4n^2}\sum_{i=1}^{n}D(X_{i}^2)+\frac{1}{16n^2}\sum_{i=1}^{n}D(Y_{i}^2) = \frac{\sigma^4}{n}  
\end{align*}

\begin{displaymath}
    \lim_{x \to +\infty} \int_{x}^{2x} \sin\frac{1}{x+t}\mathrm{d}t = \lim_{x \to +\infty}\int_{2x}^{3x}\sin\frac{1}{u} \mathrm{d}u \quad \underrightarrow{\sin\frac{1}{u} \sim \frac{1}{u}+o(\frac{1}{u})} = \ln(\frac{3}{2}) 
\end{displaymath}

\begin{align*}
    \mathrm{e}^{x} = \sum_{k=0}^{\infty} \frac{x^{k}}{k!} = \sum_{k=0}^{\infty}\left(\frac{x^{2k-1}}{(2k-1)!}+\frac{x^{2k}}{(2k)!}\right) = \sum_{k=0}^{\infty}\frac{x^{2k-1}}{(2k-1)!}+\sum_{k=0}^{\infty}\frac{x^{2k}}{(2k)!} \\ 
    \lim_{n \to \infty} \sum_{i=1}^{4}\sum_{k=0}^{n} \frac{1}{(ik)!} = \sum_{k=0}^{n} \frac{1}{(k)!} + \sum_{k=0}^{n} \frac{1}{(2k)!} + \sum_{k=0}^{n} \frac{1}{(3k)!} + \sum_{k=0}^{n} \frac{1}{(4k)!} \\ 
    = \mathrm{e}+\frac{\mathrm{e}+\mathrm{e}^{-1}}{2}+\frac{\mathrm{e}}{3}+\frac{2}{3}\cos{\frac{\sqrt{3}}{2}}\mathrm{e}^{-\frac{1}{2}} + \frac{\mathrm{e}+\mathrm{e}^{-1}}{4}+\frac{\cos 1}{2} \\ 
    = \frac{2}{3}\cos{\frac{\sqrt{3}}{2}}\mathrm{e}^{-\frac{1}{2}} + \frac{\cos 1}{2} + \frac{3}{4}\mathrm{e}^{-1}+\frac{25}{12}\mathrm{e} 
\end{align*}



\end{document}




    