%!TEX program = pdflatex
\documentclass{article}
\usepackage{amsmath}
\usepackage{bm}
\usepackage{array,tabularx} 
\usepackage{amssymb}
% \usepackage{txfonts}
\begin{document}
\begin{align*}
    \lim_{n \to \infty} n\frac{\left(\sum_{k=1}^{n}\sqrt{k}\right)^2}{\left(\sum_{k=1}^{n}\sqrt[3]{k}\right)^3}+\sum_{k=1}^{n-1}\left[\ln\left(1+\frac{1}{n+k}\right)\sin\left(\ln\left(1+\frac{k}{n}\right)\right)\right] = \\ 
    \lim_{n \to \infty} \frac{\left(\frac{1}{n}\sum_{k=1}^{n}\sqrt{\frac{k}{n}}\right)^2}{\left(\frac{1}{n}\sum_{k=1}^{n}\sqrt[3]{\frac{k}{n}}\right)^3} + \frac{1}{n}\sum_{k=1}^{n-1}\frac{1}{1+\frac{k}{n}}\sin \left(\ln\left(1+\frac{k}{n}\right)\right) = \\
    \lim_{n \to \infty} \frac{\left(\int_{0}^{1}x^{\frac{1}{2}}\mathrm{d}x\right)^2}{\left(\int_{0}^{1}x^{\frac{1}{3}}\mathrm{d}x\right)^3} + \int_{0}^{1}\frac{\sin(\ln(1+x))}{1+x} \mathrm{d}x = \frac{\frac{4}{9}}{\frac{27}{64}} + \int_{0}^{1}\sin(\ln(1+x))\mathrm{d}(\ln(x+1)) = \\ 
    \frac{256}{243} - \cos u |_{0}^{\ln 2} = \frac{499}{243} - \cos(\ln 2) \\ 
    p(x) = \frac{\mathrm{d}^{n}}{\mathrm{d}x^{n}}(1-x^m)^{n} = \left(\sum_{k=0}^{n}C_{n}^{k}(-x^m)^{k}\right)^{(n)} = \left(1+C_{n}^{1}(-x^{m})+C_{n}^{2}(-x^{m})^2+...\right)^{(n)} \\
    \exists k_{0} \in \{1,2,3,...\},mk_{0} > n \\  
    \int_{0}^{\frac{\pi}{2}} \ln\left[\left(\sin^{2}x+99\cos^{2}x\right)\left(999\sin^{2}x+\cos^{2}x\right)\right] \mathrm{d}x \\
    \left\{
        \begin{array}{rl}
            x^2+y^2 = z \\
            y = x\tan z \\ 
        \end{array}
    \right. =  
    \left\{
        \begin{array}{rl}
            x = \sqrt{\theta} \cos \theta \\
            y = \sqrt{\theta} \sin \theta \\
            z = \theta 
        \end{array} , \theta \in (0,c)
    \right.\\ 
    s = \int\mathrm{d}s = \int_{0}^{c} \sqrt{\left(\frac{\cos \theta}{2\sqrt{\theta}}-\sqrt{\theta}\sin \theta\right)^2+\left(\frac{\sin \theta}{2\sqrt{\theta}}+\sqrt{\theta}\cos \theta\right)^2+1} \mathrm{d}\theta = \\
    \int_{0}^{c} \sqrt{\frac{1}{4\theta}+\theta+1}\mathrm{d}\theta = \int_{0}^{c}\frac{2\theta+1}{2\sqrt{\theta}}\mathrm{d}\theta = \frac{2}{3}\theta^{\frac{3}{2}}+\theta^{\frac{1}{2}}|_{0}^{c} = \frac{2}{3}c^{\frac{3}{2}}+c^{\frac{1}{2}} = \sqrt{c}\left(\frac{2c}{3}+1\right) \\ 
    f(x) = \sec x , x \in (-\frac{\pi}{4},\frac{\pi}{4}) \\
    S(x) = \frac{a_{0}}{2} + \sum_{n=1}^{\infty}a_{n}\cos 4nx \\
    a_{0} = \frac{8}{\pi}\int_{0}^{\frac{\pi}{4}} \sec x \mathrm{d}x = \frac{8}{\pi}\ln|\sec x + \tan x| |_{0}^{\frac{\pi}{4}} = \frac{8}{\pi}\ln(\sqrt{2}+1) \\ 
    a_{n} = \frac{8}{\pi}\int_{0}^{\frac{\pi}{4}} \sec x \cos 4nx \mathrm{d}x = \frac{4}{n\pi}\int_{0}^{\frac{\pi}{4}} \frac{\mathrm{d}(\sin 4nx)}{\cos x} = \frac{4\sin 4nx}{n\pi\cos x} |_{0}^{\frac{\pi}{4}} - \frac{4}{n\pi}\int_{0}^{\frac{\pi}{4}}\sin 4nx \sec x \tan x \mathrm{d}x  = \\
   \end{align*}
\begin{align*}
    2m = n , \frac{x^2}{2}-\frac{\sqrt{2}xy}{m}+\frac{3y^2}{2m} = 1 \\
    A = \left[
        \begin{array}{cc}
            \frac{1}{2} & \frac{-\sqrt{2}}{2m} \\
            \frac{-\sqrt{2}}{2m} & \frac{3}{2m} \\  
        \end{array}
    \right] \quad \left(x,y\right)^{T} = Q \left(u,v\right)^{T} \\ 
    |\lambda E - A| = (\lambda-\frac{1}{2})(\lambda-\frac{3}{2m})-\frac{1}{2m^2} = \lambda^2-\frac{m+3}{2m}\lambda+\frac{3m-2}{4m^2} = 0 \\
    \lambda = \frac{\frac{m+3}{2m} \pm \sqrt{\left(\frac{m+3}{2m}\right)^2-4\frac{3m-2}{4m^2}}}{2} \notin Z \\ 
\end{align*}
\clearpage
\begin{align*}
    \lim_{x \to 0} \frac{\int_{0}^{x}t\cos t\mathrm{d}t - 1 + \cos x }{\sqrt{1+x\tan x}-\sqrt{1+x\sin x}} = \\
    \lim_{x \to 0} \frac{2(\int_{0}^{x}t\cos t\mathrm{d}t-1+\cos x)}{x(\tan x -\sin x)} = \lim_{x \to 0 }\frac{2(x\cos x-\sin x)}{2x^3} = -\frac{1}{3} \\
    \sum_{n=0}^{\infty} \frac{n^2+1}{(\frac{1}{2})^n n!} x^{n} = \sum_{n=0}^{\infty}\frac{n^2 (2x)^{n}}{n!} + \sum_{n=0}^{\infty}\frac{(2x)^n}{n!} \\
    \lim_{n \to \infty} \frac{u_{n+1}}{u_{n}} = \lim_{n \to \infty} 2\frac{(n+1)^2+1}{(n^2+1)(n+1)} = 0, x \in (-\infty,+\infty) \\
    S(x) = \sum_{n=1}^{\infty}\frac{n(2x)^n}{(n-1)!} + \mathrm{e}^{2x} = \sum_{n=0}^{\infty}\frac{(n+1)(2x)^{n+1}}{n!}+\mathrm{e}^{2x} = \sum_{n=0}^{\infty}\frac{(2x)^{n+2}}{n!}+\sum_{n=0}^{\infty}\frac{(2x)^{n+1}}{n!} + \mathrm{e}^{2x} \\
    = (4x^2+2x+1)\mathrm{e}^{2x} , x \in (-\infty,+\infty) \\  
    \left\{
        \begin{array}{rl}
            x + y - z = \mathrm{e}^{z} \\
            x\mathrm{e}^{x} = \tan t \\
            y = \cos t \\ 
        \end{array}
    \right. \\ 
    x'\mathrm{e}^x+x\mathrm{e}^{x}x'=\sec t \rightarrow \mathrm{e}^{x}(x'+x'x) = \sec t , \mathrm{e}^{x}(x'+x'x+x''+x''x+x'x') = \sec t \tan t \\ 
    y' = -\sin t , y'' = -\cos t\\
    x'+y'-z'=\mathrm{e}^{z}z' \rightarrow z' = \frac{x'+y'}{\mathrm{e}^{z}+1} \\ 
    t = 0 , x = 0 , y =  1 , z = 0 ,x' = 1,y'=0,z' = \frac{1}{2} \\
    1+0+x''+0+1= 0,x''=-2, y'' = -1 \\  
    z'' = \frac{(x''+y'')(\mathrm{e}^{z}+1)-(x'+y')(\mathrm{e}^{z}z')}{(\mathrm{e}^{z}+1)^2} = \frac{-3*2-\frac{1}{2}}{4} = -\frac{13}{8}\\
    \iint_{D}r^2\sin \theta \sqrt{1-r^2\cos (2\theta)}\mathrm{d}\sigma , D = \{(r,\theta),0 \le r \le \sec \theta,0 \le \theta \le \frac{\pi}{4}\} \\
    D = \{(x,y),0 \le y \le x , 0 \le x \le 1\} \\ 
    \iint_{D} y\sqrt{1-x^2+y^2}\mathrm{d}\sigma = \frac{1}{2} \int_{0}^{1} \int_{1-x^2}^{x^2+1-x^2} \sqrt{1-x^2+y^2} \mathrm{d}(y^2+1-x^2)\mathrm{d}x = \frac{1}{3} \int_{0}^{1} u^{\frac{3}{2}}|_{1-x^2}^{1} \mathrm{d}x\\
    = \frac{1}{3}\int_{0}^{1} 1-(1-x^2)^{\frac{3}{2}} \mathrm{d}x = \frac{1}{3} - \int_{0}^{\frac{\pi}{2}} \cos^4 t\mathrm{d}t = \frac{1}{3} - \frac{1*3*1*\pi}{3*4*2*2} = \frac{1}{3} - \frac{\pi}{16} \\
    u = ax^2+by^2+cz^2 , x+y+z=1 , (ax^2+by^2+cz^2)(\frac{1}{a}+\frac{1}{b}+\frac{1}{c}) \ge (x+y+z)^2 = 1 \\
    \min_{x>0,y>0,z>0} {u(x,y,z)} = \frac{1}{\frac{1}{a}+\frac{1}{b}+\frac{1}{c}}\\ 
\end{align*}
    

\clearpage
\begin{align*}
    a_{n} = \int_{0}^{1} \frac{x^{n-1}}{1+x}\mathrm{d}x = \int_{0}^{1} x^{n-1}\mathrm{d}(\ln(x+1)) = x^{n-1}\ln(x+1)|_{0}^{1} - (n-1)\int_{0}^{1}\ln(x+1)x^{n-2}\mathrm{d}x\\ 
    a_{n} = \frac{1}{n}\int_{0}^{1}\frac{\mathrm{d}(x^n)}{1+x} = \frac{x^n}{n(1+x)}|_{0}^{1} + \int_{0}^{1}\frac{x^n\mathrm{d}x}{n(1+x)^2} = \frac{1}{2n} + \int_{0}^{1}\frac{\mathrm{d}(x^{n+1})}{(1+x)^2 n(n+1)} =\\ 
    \frac{1}{2n} + \frac{x^{n+1}}{(1+x)^2 n(n+1)}|_{0}^{1} + \int_{0}^{1}\frac{2x^{n+1}\mathrm{d}x}{(n+1)(1+x)^3} = \frac{1}{2n} + \frac{1}{4n^2}+o(\frac{1}{n^2}) m n \to \infty \\ 
    I_{1} = \iint_{S} \frac{xz}{a^2}\mathrm{d}y\mathrm{d}z+\frac{yz}{b^2}\mathrm{d}z\mathrm{d}x+\frac{z^2}{c^2} \mathrm{d}x\mathrm{d}y\\
    I_{2} = 0 , S_{1} = \{(x,y,z),\frac{x^2}{a^2}+\frac{y^2}{b^2} \le 1,z = 0 \},down0 \\
    D_{xy} = \{(x,y),\frac{x^2}{a^2}+\frac{y^2}{b^2} \le 1\} \\
    I_{1}+I_{2} = \left(\frac{1}{a^2}+\frac{1}{b^2}+\frac{2}{c^2}\right) \iiint_{\Omega} z\mathrm{d}v = \left(\frac{1}{a^2}+\frac{1}{b^2}+\frac{2}{c^2}\right)\frac{c^2}{2}\iint_{D_{xy}} \left(1-\frac{x^2}{a^2}-\frac{y^2}{b^2}\right)\mathrm{d}\sigma \\
    \frac{x}{a} = u , \frac{y}{b} = v ,J = ab \\
    I_{1}+I_{2} = \left(\frac{1}{a^2}+\frac{1}{b^2}+\frac{2}{c^2}\right)\frac{c^2}{2}ab \iint_{D_{uv}}(1-u^2-v^2)\mathrm{d}\sigma \\ 
    \iint_{D_{uv}}(1-u^2-v^2)\mathrm{d}\sigma = \int_{0}^{1}(1-r^2)r\mathrm{d}r\int_{0}^{2\pi}\mathrm{d}\theta = \frac{\pi}{2} \\
    I_{1} = \left(\frac{1}{a^2}+\frac{1}{b^2}+\frac{2}{c^2}\right)\frac{c^2\pi}{4}ab  \\ 
\end{align*}
    
\end{document}