%!TEX program = pdflatex
\documentclass{article}
\usepackage{amsmath}
\usepackage{bm}
\usepackage{array,tabularx} 
\usepackage{amssymb}
\usepackage{tikz}
\usepackage{tikz-qtree}
% \usepackage{txfonts}
\begin{document}

\begin{align*}
    \lim_{n \to \infty}\sum_{k=1}^{n} k(1-p)^{k-1} p = 3 \\
    p\sum_{k=1}^{n}kq^{k-1} = pf(q) = (1-q)f(q) = g(q)\\
    f(q) = \frac{g(q)}{1-q} \quad \underrightarrow{integral} \quad \int f(q) \mathrm{d}q = \int \frac{g(q)}{1-q}\mathrm{d}q\\
    \sum_{k=1}^{n}q^{k} = \frac{q}{1-q} = \int \frac{g(q)}{1-q}\mathrm{d}q \quad \underrightarrow{derivation} \quad \frac{(1-q)+q}{(1-q)^2} = \frac{g(q)}{1-q}\\
    p = \frac{1}{3} \\ 
    \lim_{n \to \infty}\sum_{k=2}^{n} k[(1-p)^{k-1}p + p^{k-1}(1-p)] = 3 \\ 
    G(p) = p\sum_{k=2}^{n}k(1-p)^{k-1} + (1-p)\sum_{k=2}^{n}kp^{k-1} \\
    F(x) = (1-x)\sum_{k=2}^{n}kx^{k-1} \\ \frac{F(x)}{1-x} = \sum_{k=2}^{n}kx^{k-1} \quad \underrightarrow{integral} \quad \\
    \int \frac{F(x)}{1-x} \mathrm{d}x = \frac{x^2}{1-x} \quad \underrightarrow{derivation} \quad \frac{F(x)}{1-x} = \frac{2x(1-x)+x^2}{(1-x)^2}\\
    F(x) = \frac{(2-x)x}{1-x}, \quad G(p) = F(1-p) + F(p) = \frac{(1-p)(1+p)}{p} + \frac{(2-p)p}{1-p} = 3\\
    p = \frac{1}{2} \\ 
\end{align*}


\begin{align*}
    % f(x,y) = \frac{1}{2}\mathrm{e}^{-y}, y> |x| , x \in (-\infty,+\infty) \\
    f(x,y) = \left\{ 
    \begin{array}{rl} 
        \frac{1}{2}\mathrm{e}^{-y}, y> |x| , x \in (-\infty,+\infty)\\
        0, others \\ 
    \end{array} \right.  \\ \\
    f_{X}(x) = \int_{|x|}^{+\infty} \frac{1}{2}\mathrm{e}^{-y}\mathrm{d}y = -\frac{1}{2}\mathrm{e}^{-y} |_{|x|}^{+\infty} = \frac{1}{2}\mathrm{e}^{-|x|}, x \in (-\infty,+\infty)  \\
    % f_{Y}(y) = \int_{-y}^{+y} \frac{1}{2}\mathrm{e}^{-y}\mathrm{d}x = \frac{1}{2}\mathrm{e}^{-y} \cdot 2y = y\mathrm{e}^{-y}, y \in (0,+\infty) \\
    % f_{Y}(y) = 0, y \in (-\infty,0) \\
    f_{Y}(y) = \left\{ 
    \begin{array}{rl} 
        \int_{-y}^{+y} \frac{1}{2}\mathrm{e}^{-y}\mathrm{d}x = \frac{1}{2}\mathrm{e}^{-y} \cdot 2y = y\mathrm{e}^{-y}, y \in (0,+\infty) \\
        0, y \in (-\infty,0) \\
    \end{array} \right. \ \\ 
    \\
    obviously \quad f(x,y) \neq f_{X}(x) \cdot f_{Y}(y) \\
    f_{Y|X}(y|x) = \frac{f(x,y)}{f_{X}(x)} = \frac{\frac{1}{2}\mathrm{e}^{-y}}{\frac{1}{2}\mathrm{e}^{-|x|}} = \mathrm{e}^{-y+|x|}, y \in (|x|,+\infty)\\
    \\
    f(x,y) = \left\{ 
    \begin{array}{rl} 
        \frac{1}{x}\mathrm{e}^{-2x}, y \in (0,2x), x \in (0,+\infty)\\
        0, others \\ 
    \end{array} \right.  \\
    \left\{
        \begin{array}{rl} 
        U = 2X\\
        V = X+Y \\ 
        \end{array}\right. \rightarrow \left\{
            \begin{array}{rl} 
            X= \frac{1}{2}U + 0 \cdot V\\
            Y = -\frac{1}{2}U +V\\ 
            \end{array}\right. \\
    \\
    J = \left| \begin{array}{cc} 
        \frac{\partial X}{\partial U} & \frac{\partial X}{\partial V} \\ 
        \\
        \frac{\partial Y}{\partial U} & \frac{\partial Y}{\partial V} \\
    \end{array}
        \right| =\left| \begin{array}{cc} 
        \frac{1}{2} & 0 \\ 
        \\
        -\frac{1}{2} & 1 \\
    \end{array}
        \right| = \frac{1}{2}\\
        \\
        \frac{u}{2} \in (0,+\infty) , -\frac{u}{2}+v \in (0,u)\\
        g(u,v) = f(\frac{u}{2},-\frac{u}{2}+v)|J| = \frac{2}{u}\mathrm{e}^{-u} \cdot \frac{1}{2} = \frac{\mathrm{e}^{-u}}{u} , u \in (0,+\infty), v \in (\frac{u}{2},\frac{3u}{2})\\
        g(u,v) = 0, others\\
        \\
        Y \sim U(0,1)\\
    F_{Y}(y) = P(Y <= y) = P (g(X) <= y)  = F_{X}(g^{-1}(y)) \\
    F_{Y}(y) = F_{X}(F^{-1}(y)) = y  , y \in (0,1) \
\end{align*}

\begin{align*}
    \mathrm{Pr}[X=k] = \frac{2^{k-1}+2}{3^k} \\ 
    \mathrm{Ex}[X] = \lim_{n \to \infty} \sum_{k=2}^{n} \mathrm{Pr}[X=k] \cdot k = \sum_{k=2}^{\infty} \left[\frac{1}{2}\left(\frac{2}{3}\right)^k k + 2 \left(\frac{1}{3}\right)^k k \right] \\ 
    = \frac{1}{2} \left(\frac{\frac{2}{3}}{\left(1-\frac{2}{3}\right)^2} - \frac{2}{3}\right) + 2\left(\frac{\frac{1}{3}}{\left(1-\frac{1}{3}\right)^2}-\frac{1}{3}\right) = \frac{7}{2} = 3.5\\
\end{align*}

\begin{align*}
    x^2+y^2 = 1, \quad x+\frac{1}{y+2} \in \quad ? \\ 
    = \cos \theta + \frac{1}{\sin \theta + 2}, \quad \theta \in [0,2\pi] \\
    f(\theta) = F(x(\theta),y(\theta)) \\
    f'(\theta) = -\sin \theta-\frac{\cos \theta}{(\sin \theta +2)^2} = -\cos \theta \left(\tan \theta+\frac{1}{(\sin \theta +2)^2} \right)\\
    \frac{xy+2x+1}{y+2}\\
    2x+2y(x)y'(x)=0, y'(x) = -\frac{x}{y(x)} , y(x) \neq 0\\
    F(x) = x + \frac{1}{y(x)+2}, F'(x) = 1-\frac{y'(x)}{(y(x)+2)^2}\\
    F'(x) = 1 + \frac{x}{y(x)(y(x)+2)^2}\\
\end{align*}

\clearpage

\begin{align*}
    \mathbf{!!!Error \quad Expand!!!} \\
    X_{1}, X_{2}, Y > 0 \\
    F_{X_{1}}(x) = 1-\mathrm{e}^{-\lambda_{1} x}, F_{X_{2}}(x) = 1-\mathrm{e}^{-\lambda_{2} x}, F_{Y}(y) = 1-\mathrm{e}^{-\mu y}\\
    f_{X_{1}}(x) = \lambda_{1} \mathrm{e}^{-\lambda_{1} x}, f_{X_{2}}(x) = \lambda_{2} \mathrm{e}^{-\lambda_{2} x}, f_{Y}(y) = \mu \mathrm{e}^{-\mu y}\\
    F_{X}(x) = P\{X \le x\} = P\{X \le x, Y \le X_{1}\} + P\{X \le x, Y > X_{1}\}\\
    = P\{X \le x | Y \le X_{1}\} P\{Y \le X_{1}\} + P\{X \le x | Y > X_{1}\} P\{Y > X_{1}\}\\
    = P\{X_{1} \le x\}P\{Y \le X_{1}\} + P\{X_{1}+X_{2} \le x\}P\{Y > X_{1}\}\\
    = F_{X_{1}}(x)P\{Y-X_{1} \le 0\} + P\{X_{1}+X_{2} \le x\} P\{Y-X_{1} > 0\} \\
    Z = Y-X_{1} \\
    Y = Z + X_{1}, \quad  y \in (z,z+x), x \in (0,+\infty) \\
    F_{Z}(z) = P\{Z \le z\} = P\{Y-X_{1} \le z\} = \iint_{Y-X_{1} \le z}f(x_{1},y) \mathrm{d}x_{1}\mathrm{d}y\\ 
    = \int_{z}^{z+x} \int_{0}^{+\infty} f(x_{1},y) \mathrm{d}x_{1}\mathrm{d}y = \int_{z}^{z+x} \int_{0}^{+\infty} f_{X_{1}}(x_{1})f_{Y}(y) \mathrm{d}x_{1}\mathrm{d}y\\
    = \frac{\mu}{\lambda_{1}+\mu} \mathrm{e}^{-\mu z}, \quad z \in (0,+\infty) \\
    P\{Y-X_{1} \le 0\} = F_{Z}(0) = \frac{\mu }{\lambda_{1}+\mu}, P\{Y-X_{1} > 0\} = \frac{\lambda_{1}}{{\lambda_{1}+\mu}}\\
    W = X_{1}+X_{2} \\ 
    X_{2} = W-X_{1}, \quad v \in (0, w-u), u \in (0,w)\\ 
    F_{W}(w) = P\{W \le w\} = P\{X_{1}+X_{2} \le w\} = \int_{0}^{w}f_{X_{1}}(u)\left[\int_{0}^{w-u} f_{X_{2}}(v)\mathrm{d}v\right] \mathrm{d}u\\
    = 1 - \frac{\lambda_{2}}{\lambda_{2}-\lambda_{1}} \mathrm{e}^{-\lambda_{1}w} + \frac{\lambda_{1}}{\lambda_{2}-\lambda_{1}} \mathrm{e}^{-\lambda_{2}w}, \quad w \in (0,+\infty)\\
    F_{X}(x) = \left(1-\mathrm{e}^{-\lambda_{1} x}\right) \cdot (\frac{\mu}{\lambda_{1}+\mu}) + \left(1 - \frac{\lambda_{2}}{\lambda_{2}-\lambda_{1}} \mathrm{e}^{-\lambda_{1}x} + \frac{\lambda_{1}}{\lambda_{2}-\lambda_{1}} \mathrm{e}^{-\lambda_{2}x}    \right)\cdot(\frac{\lambda_{1}}{\lambda_{1}+\mu})\\
    \\
\end{align*}


\begin{align*}
    max(X_{1},X_{2}) = \left\{ 
        \begin{array}{rl}
            X, \quad X \ge Y \\
            Y, \quad X < Y
        \end{array}
    \right. \longrightarrow \\
    max(X_{1},X_{2}) = \frac{X_{1} + X_{2} + |X_{1}-X_{2}|}{2}\\
    X_{1} \sim (a, \sigma^{2}), \quad X_{2} \sim (a, \sigma^{2})\\
    E(X_{1}-X_{2}) = E(X_{1}-X_{2}) = E(X_{1})-E(X_{2}) = a-a=0\\
    D(X_{1}-X_{2}) = D(X_{1}) + D(X_{2}) = 2\sigma^{2} \\
    X_{1}-X_{2} \sim (0,2\sigma^{2}) \longrightarrow \\
    f_{X_{1}-X_{2}}(x) = \frac{1}{\sqrt{2\pi}\sqrt{2}\sigma}\mathrm{e}^{-\frac{x^2}{2 \cdot 2\sigma^{2}}}, \quad x \in (-\infty,+\infty)\\
    Z = X_{1}-X_{2}\\
    E\{|X_{1}-X_{2}|\} = E\{X_{1}-X_{2},X_{1} \ge X_{2}\} +E\{X_{2}-X_{1}, X_{1} < X_{2}\}\\
    \mathrm{because \quad of \quad symmetric}\\
    E\{Z| z \ge 0\}  + E\{-Z | z < 0\} = 2 E\{Z| z \ge 0\} \\ 
    = 2 \int_{0}^{+\infty} \frac{1}{\sqrt{2\pi}\sqrt{2}\sigma}\mathrm{e}^{-\frac{z^2}{2 \cdot 2\sigma^{2}}} \mathrm{d}z \\
    = \int_{0}^{+\infty} \frac{2\sigma}{\sqrt{\pi}} \mathrm{e}^{-\frac{z^2}{4\sigma^{2}}} \mathrm{d}\left(\frac{z^2}{4\sigma^{2}}\right) = \frac{2\sigma}{\sqrt{\pi}}\\
    E\{max(X_{1},X_{2})\} = E\{\frac{X_{1} + X_{2} + |X_{1}-X_{2}|}{2}\} \\ 
    = \frac{1}{2} \cdot E\{X_{1}\} + \frac{1}{2} \cdot E\{X_{2}\} + \frac{1}{2} E\{|X_{1} - X_{2}|\} \\
    = \frac{1}{2} a + \frac{1}{2} a + \frac{1}{2} \frac{2\sigma}{\sqrt{\pi}} = a+\frac{\sigma}{\sqrt{\pi}}\\
\end{align*}

\end{document}