%!TEX program = pdflatex
\documentclass{article}
\usepackage{amsmath}
\usepackage{bm}
\usepackage{array,tabularx} 
\usepackage{amssymb}
% \usepackage{txfonts}
\begin{document}

\begin{align*}
    \mathbf{Traditional \quad Probability \quad Theory} \\ 
    \mathbf{Opposition}: P(A)+P(\bar{A}) = 1 \quad \mathbf{Exclusive}: A\cap B = \varnothing \Rightarrow P(AB)=0\\ 
    \mathbf{Independent}: P(AB) = P(A)P(B) \quad \mathbf{Equal}: A = B \Rightarrow P(A) = P(B)\\ 
    A - B = A\bar{B} = A \cap \bar{B} \Rightarrow P(A-B) = P(A) - P(AB) \\ 
    P(A \cup B \cup C) = P(A)+P(B)+P(C)-P(BC)-P(AC)-P(AB)+P(ABC) \\ 
    P(B|A) = \frac{P(AB)}{P(A)} \quad P(A_{1}A_{2}...A_{n}) = P(A_{1})P(A_{2}|A_{1})P(A_{3}|A_{1}A_{2})...P(A_{n}|A_{1}...A_{n-1}) \\
    \mathbf{Bayes} \quad P(B_{j}|A) = \frac{P(A|B_{j})P(B_{j})}{\sum_{i=1}^n P(A|B_{i})P(B_{i})}\\  
\end{align*}


$\mathbf{Random \quad Variable \quad Digital \quad Properties \quad }$ \\ 
\begin{tabular}{|c|c|c|c|c|}%
    \hline 
    Distr & Mark & EX & DX & Addition \\ 
    \hline 
    Bin & $B(n,p)$ & $np$ & $np(1-p)$ & $P\{X=k\}$ = $\mathbf{C_{n}^k}(1-p)^{n-k}p^k$ \\ 
    \hline 
    Poi & $\pi(\lambda)$ & $\lambda$ & $\lambda$ & $P\{X=k\} = \frac{\lambda^k}{k!}\mathrm{e}^{-\lambda}, k = 0,1,2,...$  \\ 
    \hline 
    Geo & $G(p)$ & $\frac{1}{p}$ & $\frac{1-p}{p^2}$ & $P\{X=k\} = (1-p)^{k-1}p,k=1,2,...$ \\ 
    \hline 
    Hyp & $H(n,M,N)$ & $\frac{nM}{N}$ & $\frac{nM}{N}(1-\frac{M}{N})(\frac{N-n}{N-1})$ & $P\{X=i\} = \frac{\mathbf{C}_{M}^{i}\mathbf{C}_{N-M}^{n-i}}{\mathbf{C}_{N}^{n}}$ \\ 
    \hline 
    Uni & $U(a,b)$ & $\frac{a+b}{2}$ & $\frac{(b-a)^2}{12}$ & \\ 
    \hline 
    Exp & $E(\lambda)$ & $\frac{1}{\lambda}$ & $\frac{1}{\lambda^2}$ & \\ 
    \hline 
    Nor & $N(\mu,\sigma^2)$ & $\mu$ & $\sigma^2$ & \\ 
    \hline 
\end{tabular}

\begin{align*} 
    \mathbf{Uni} : f(x) = \left\{
        \begin{array}{rl}
            \frac{1}{b-a}, a \le x \le b \\
            0, others   
        \end{array} \right.\ \quad F(x) = \left\{
        \begin{array}{rl}
            0, x < a\\ 
            \frac{x-a}{b-a}, a \le x < b \\
            1, x \ge b    
        \end{array} \right.\ \\
    \mathbf{Exp} : f(x) = \left\{
        \begin{array}{rl}
            \lambda\mathrm{e}^{-\lambda x}, x > 0 \\
            0, x \le 0    
        \end{array} \right.\ \quad F(x) = \left\{
        \begin{array}{rl}
            1-\mathrm{e}^{-\lambda x}, x > 0\\ 
            0, x \le 0 
        \end{array} \right.\ \\
    \mathbf{Nor}: f(x) = \frac{1}{\sqrt{2\pi}\sigma}\mathrm{e}^{-\frac{(x-\mu)^2}{2\sigma^2}} , F(x) = \int_{-\infty}^{x} f(t)\mathrm{d}t,x \in (-\infty,+\infty)  \\ 
    f(\mu+x) = f(\mu-x),F(\mu+x)+F(\mu-x)=1,F(\mu)=\frac{1}{2} \\
    X \sim N(0,1),\phi(x) = \frac{1}{\sqrt{2\pi}}\mathrm{e}^{-\frac{x^2}{2}},\Phi(x) = \int_{-\infty}^{x}\phi(t)\mathrm{d}t \\ 
    \phi(-x) = \phi(x),\quad \Phi(a)+\Phi(-a) = 1,\Phi(0)=\frac{1}{2}, \quad F(x) = \Phi\left(\frac{x-\mu}{\sigma}\right)\\  
    f(x,y) \ge 0 \quad \int_{-\infty}^{\infty}\int_{-\infty}^{\infty}f(x,y)\mathrm{d}x\mathrm{d}y = 1\\ 
    f_{X}(x) = \int_{-\infty}^{\infty}f(x,y)\mathrm{d}y > 0 \quad f_{Y}(y) = \int_{-\infty}^{\infty}f(x,y)\mathrm{d}x > 0 \\ 
    f_{X|Y}(x|y) = \frac{f(x,y)}{f_{Y}(y)}, f_{Y|X}(y|x) = \frac{f(x,y)}{f_{X}(x)} \\ 
    \mathbf{Discrete}: P\{Z=g(x_{i},y_{j})\} = P\{X=x_{i},Y=y_{j}\} = P_{ij} \\ 
    F_{Z}(z)=P\{Z \le z\} = P\{ g(X,Y) \le z \} = \sum_{g(x_{i},y_{j})\le z} P\{X=x_{i},Y=y_{j}\} \\ 
    \mathbf{Continuous} : Z = g(X,Y) \quad F_{Z}(z)=P\{Z\le z\} = P\{g(X,Y)\le z\} = \iint_{g(x,y)\le z}f(x,y)\mathrm{d}x\mathrm{d}y \\
    Z=\max(X,Y),F_{\max}(z)=F_{X}(z)F_{Y}(z) \quad Z=\min(X,Y),F_{\min}(z)=1-[1-F_{X}(z)][1-F_{Y}(z)] \\ 
    Z_{1}=\max(X,Y) = \frac{X+Y+|X-Y|}{2} \quad Z_{2}=\min(X,Y)=\frac{X+Y-|X-Y|}{2} \quad Z_{1}Z_{2}=XY \\ 
    (X,Y) \sim U(D), 
    f(x,y) = \left\{ 
    \begin{array}{rl} 
        \frac{1}{S_{D}}, (x,y) \in D\\ 
        0, others
    \end{array} \right. \ \\ 
    (X,Y) \sim N(\mu_{1},\mu_{2};\sigma_{1},\sigma_{2},\rho),f(x,y) = \frac{1}{2\pi \sigma_{1} \sigma_{2} \sqrt{1-\rho^2}} \mathrm{e}^{-\frac{1}{2(1-\rho^2)}[(\frac{x-\mu_{1}}{\sigma_{1}})^2-\frac{2\rho (x-\mu_{1})(y-\mu_{2})}{\sigma_{1}\sigma_{2}}+(\frac{y-\mu_{2}}{\sigma_{2}})^2]} \\
\end{align*}

\clearpage

\begin{align*}
    F(x) = P\{X \le x\} = \int_{-\infty}^{x} f(x) \mathrm{d}x \\ 
    F(x,y) = P\{X \le x,Y \le y\} = \int_{-\infty}^{x}\int_{-\infty}^{y}f(u,v)\mathrm{d}v\mathrm{d}u \\
    1 = \sum_{i=1}^{\infty} x_{i}p_{i} \quad 1 = \int_{-\infty}^{+\infty}f(x)\mathrm{d}x \\ 
    E(X) = \sum_{i=1}^{\infty}x_{i}p_{i} \quad E(X) = \int_{-\infty}^{+\infty}xf(x)\mathrm{d}x \\  
    E[g(X)] = \sum_{i=1}^{\infty}g(x_{i})p_{i} \quad E[g(X)] = \int_{-\infty}^{+\infty}g(x)f(x)\mathrm{d} x \\
    E[g(X,Y)] = \sum_{j=1}^{\infty}\sum_{i=1}^{\infty}g(x_{i},y_{j})P_{ij} \quad E[g(X,Y)] = \int_{-\infty}^{+\infty}\int_{-\infty}^{+\infty}g(x,y)f(x,y)\mathrm{d}x\mathrm{d}y \\ 
    \exists X \sim F(x) ,\forall X > 0 , E(X) = \int_{0}^{+\infty}(1-F(x))\mathrm{d}x = \int_{0}^{+\infty} P\{X>x\}\mathrm{d}x \\ 
    E(C) = C \quad E(CX) = CE(X) \quad E(X+C) = E(X)+C \quad E(X+Y) = E(X)+E(Y) \\ 
    D(X) = \sum_{i=1}^{n}[x_{i}-E(X)]^2p_{i} \quad D(X) = \int_{-\infty}^{+\infty}[x-E(X)]^2f(x)\mathrm{d}x \\ 
    D(X) = E(X^2)-[E(X)]^2 \quad D(C) = 0 \quad D(CX)=C^2D(X) \quad D(X+C) = D(X) \\ 
    Cov(X,Y) = E(XY) - E(X)E(Y) \quad D(X\pm Y) = D(X)+D(Y)\pm 2Cov(X,Y) \\ 
    Cov(X,Y) = Cov(Y,X) \quad Cov(X,X) = D(X) \quad Cov(X,c) = 0 \\ 
    Cov(aX,bY) = abCov(X,Y) \quad Cov(X_{1}+X_{2},Y) = Cov(X_{1},Y)+Cov(X_{2},Y) \\ 
    \rho_{XY} = \frac{E(XY)-E(X)E(Y)}{\sqrt{D(X)}\sqrt{D(Y)}}= \frac{Cov(X,Y)}{\sqrt{D(X)}\sqrt{D(Y)}} \\ 
    X \sim N(0,1) \quad E(X^{2k}) = (2k-1)!! \quad E(X^{2k-1}) = 0 , k \in \{1,2,3,...\} \\ 
\end{align*}

\begin{align*}
    \mathbf{Large \quad Number \quad Law \quad Central \quad Limit \quad Theorem } \\ 
    P \{ {|X-E(X)|\ge \epsilon} \} \le \frac{D(X)}{\epsilon^{2}} \\
    \lim_{n \to \infty}P\{|\frac{X_{n}}{n}-p| < \epsilon\} = 1 \\
    \lim_{n \to \infty}P\{|\frac{1}{n}\sum_{k=1}^nX_{k}-\mu|<\epsilon\} = 1 \\
    \lim_{n \to \infty}P\{|\frac{1}{n}\sum_{k=1}^n X_{k} - \frac{1}{n}\sum_{k=1}^n E(X_{k})| < \epsilon\} = 1 \\ 
    \sum_{i=1}^{n}X_{i} \sim N(n\mu,n\sigma^2), \lim_{n \to \infty}P\{\frac{\sum_{i=1}^nX_{i}-n\mu}{\sqrt{n}\sigma} \le x\} = F_{n}(x) = \Phi(x) \\ 
    X \sim N(np,np(1-p)), \lim_{n \to \infty }P\{\frac{X_{n}-np}{\sqrt{np(1-p)}} \le x \} = \Phi(x) \\ 
\end{align*}

\clearpage

\begin{align*}
    \mathbf{Mathematical \quad Statistics} \\ 
    \bar{X} \sim N(\mu,\frac{\sigma^2}{n}), \frac{\bar{X}-u}{\sigma/\sqrt{n}} \sim N(0,1)\\ 
    S^2 = \frac{1}{n-1}\sum_{i=1}^n(X_{i}-\bar{X})^2 = \frac{1}{n-1}[\sum_{i=1}^nX_{i}^2 - n \bar{X}^2] \\ 
    E(S^2) = \sigma^2, D(S^2) = \frac{2\sigma^4}{n-1} \\ 
    \frac{\sum_{i=1}^n(X_{i}-\mu)^2}{\sigma^2} \sim \chi^2(n) \\ 
    \frac{\sum_{i=1}^n(X_{i}-\bar{X})^2}{\sigma^2} \sim \chi^2(n-1) \\ 
    \chi^2 \sim \chi^2(n), E(\chi^2(n)) = n, D(\chi^2(n)) = 2n \\ 
    T \sim t(n), T = \frac{X}{\sqrt{Y/n}} \frac{\sim}{\sim} \frac{N(0,1)}{\sqrt{\chi^2(n)/n}}\\
    F \sim F(n1,n2), F = \frac{X/n1}{Y/n2} \frac{\sim}{\sim} \frac{\chi^2(n1)/n1}{\chi^2(n2)/n2} \\ 
    (X,Y) \sim N(\mu_{1},\mu_{2};\sigma_{1}^2,\sigma_{2}^2,0) \\ 
    \frac{\frac{(n_{1}-1)S_{1}^2}{\sigma_{1}^2}/(n_{1}-1)}{\frac{(n_{2}-1)S_{2}^2}{\sigma_{2}^2}/(n_{2}-1)} \sim F(n_{1}-1,n_{2}-1) \\
    \frac{\frac{\sum_{i=1}^{n_{1}}(X_{i}-\mu_{1})^2}{\sigma_{1}^2}/n_{1}}{\frac{\sum_{i=1}^{n_{2}}(X_{i}-\mu_{2})^2}{\sigma_{2}^2}/n2} \sim F(n1,n2) \\  
    \frac{\bar{X}-\bar{Y}-(\mu_{1}-\mu_{2})}{\sqrt{\frac{\sigma_{1}^2}{n_{1}}+\frac{\sigma_{2}^2}{n2}}} \sim N(0,1) \\ 
    \exists \sigma_{1} = \sigma_{2}, \frac{\bar{X}-\bar{Y}-(\mu_{1}-\mu_{2})}{S_{\omega}\sqrt{\frac{1}{n_{1}}+\frac{1}{n_{2}}}} \sim t(n_{1}+n_{2}-2) \\ 
    S_{\omega} = \sqrt{\frac{(n_{1}-1)S_{1}^2+(n_{2}-1)S_{2}^2 }{n_{1}+n_{2}-2}}
\end{align*}

\clearpage

\end{document}